checkpoint: step indexed PRelN_PRel lemma

KLR/Semantics/SmallStep.lean
@@ -4,10 +4,17 @@ Released under Apache 2.0 license as described in the file LICENSE.
 Authors: Markus de Medeiros
 -/
 
-import Std.Data.HashMap
-
 /- # Mechanization of a generic nondeterministic small-step semantics -/
 
+/-- A small step semantics.
+
+Each configuration `prog × state` nondeterministically steps to anything in the `step` relation.
+We distinguish between error states and terminated states using the `to_val` partial function.
+The `val` type should include everything we want to observe about the state of our terminated programs.
+
+markusde: Having to_val be a partial function out of prog × state rather than a total function out of
+{ x : prog × state | stuck x } is more robust against changes to the semantics.
+-/
 structure SmallStep : Type _ where
   prog : Type _
   state : Type _
@@ -16,8 +23,10 @@ structure SmallStep : Type _ where
   to_val : prog × state → Option val
   value_stuck {c c' : prog × state} : (to_val c).isSome → step c c' → False
 
-class SmallStepDet (S : SmallStep) where
-  step_det c : ∃ c', ∀ c'', S.step c c'' → c'' = c'
+/-- A small step semantics is deterministic when every configuration is either stuck,
+or steps to exactly one state. -/
+class Det (S : SmallStep) where
+  step_det {c c'} : S.step c c' → ∀ c'', S.step c c'' → c'' = c'
 
 namespace SmallStep
 
@@ -32,40 +41,15 @@ inductive stepN : Nat → S.prog × S.state → S.prog × S.state → Prop where
 
 theorem stepN_zero_inv (H : S.stepN 0 c c') : c = c' := by cases H; trivial
 
+theorem stepN_one (H : S.stepN 1 c c') : S.step c c' := by
+  rcases H; rename_i _ H1 H2
+  exact (stepN_zero_inv _ H2).symm ▸ H1
+
 theorem stepN_stuck_inv (H : S.stepN m c c') (Hs : S.stuck c) : m = 0 := by
   cases H
   · rfl
   · rename_i Hstep HstepN
     exact (Hs _ Hstep).elim
-
-/-- For any of the first n steps of execution, all stuck states satisfy `Φ`. -/
-inductive satisfiesN (Φ : S.prog × S.state → Prop) : Nat → S.prog × S.state → Prop where
-| stuck : S.stuck c → Φ c → satisfiesN Φ n c
-| step  : S.step c c' → satisfiesN Φ n c' → satisfiesN Φ n.succ c
-
-/-
-theorem satisfiesN_stepN (H : S.satisfiesN Φ n c) : ∀ m, m ≤ n → S.stuck c' → S.stepN m c c' → Φ c' := by
-  revert c
-  induction n
-  · intro c H m Hm Hs Hs'
-    rw [Nat.le_zero_eq] at Hm
-    rcases H with ⟨_, H⟩
-    exact (stepN_zero_inv S (Hm▸Hs'))▸H
-  rename_i n IH
-  rintro c H m Hm Hstuck Hstep
-  cases H
-  · rename_i Hs' HΦ
-    have Hz := stepN_stuck_inv S Hstep Hs'
-    have Hc := stepN_zero_inv S (Hz ▸ Hstep)
-    exact Hc ▸ HΦ
-  rename_i _ Hsat Hstep'
-  rcases m with (_|m)
-  · exact Hstuck _ (stepN_zero_inv S Hstep ▸ Hstep') |>.elim
-  -- have Hm' := Nat.add_le_add_iff_right ▸ Hm
-  cases Hstep
-  -- apply IH Hsat _ (Nat.le_of_lt_succ Hm) Hstuck
-  sorry
--/
 
 theorem stepN_1_iff_step : S.stepN 1 (p, s) (p', s') ↔ S.step (p, s) (p', s') := by
   refine ⟨?_, (stepN.step · (stepN.done rfl))⟩
@@ -79,73 +63,6 @@ theorem step_not_stuck (H : S.step (p1, s1) (p1', s1')) : (S.to_val (p1, s1)).is
 
 end basic
 
-@[simp] abbrev prod.prog (S : SmallStep) := S.prog × S.prog
-@[simp] abbrev prod.state (S : SmallStep) := S.state × S.state
-@[simp] abbrev prod.val (S : SmallStep) := S.val × S.val
-
-inductive prod.step {S : SmallStep} : (prod.prog S) × (prod.state S) → (prod.prog S) × (prod.state S) → Prop where
-| step_l : S.step (p1, s1) (p1', s1') → prod.step ((p1, p2), (s1, s2)) ((p1, p2'), (s1, s2'))
-| step_r : S.step (p2, s2) (p2', s2') → prod.step ((p1, p2), (s1, s2)) ((p1, p2'), (s1, s2'))
-
-@[simp] def prod.to_val {S : SmallStep} (c : prod.prog S × prod.state S) : Option (prod.val S) :=
-  match S.to_val ⟨c.1.1, c.2.1⟩, S.to_val ⟨c.1.2, c.2.2⟩ with
-  | some v1, some v2 => some (v1, v2)
-  | _, _ => none
-
-theorem prod.value_stuck {S : SmallStep} {c c' : prod.prog S × prod.state S} :
-    (prod.to_val c).isSome → prod.step c c' → False := by
-  rcases c with ⟨⟨p1, p2⟩, ⟨s1, s2⟩⟩
-  simp only [to_val]
-  split
-  · rename_i Hv1 Hv2
-    intro _ Hstep; rcases Hstep with (Hs|Hs)
-    · exact S.value_stuck (Hv1▸rfl) Hs
-    · exact S.value_stuck (Hv2▸rfl) Hs
-  · simp
-
-def prod (S : SmallStep) : SmallStep where
-  prog := prod.prog S
-  state := prod.state S
-  val := prod.val S
-  step := prod.step
-  to_val := prod.to_val
-  value_stuck := prod.value_stuck
-
-/-
-
--- There is a better way
-
-
-section prod
-
-variable {S : SmallStep}
-
-
-/-- Every n-step trace in the product semantics can be thought of as two traces in the semantics
-of the components. -/
-theorem prod.step_noninterference {n : Nat} :
-    S.prod.stepN n ((p, q), (s, t)) ((p', q'), (s', t')) ↔
-    (∃ mₗ mᵣ : Nat, n = mₗ + mᵣ ∧ S.stepN mₗ (p, s) (p', s') ∧ S.stepN mᵣ (q, t) (q', t')) :=
-  sorry
-
-def prod.π₁ (s : S.prod.prog × S.prod.state) : S.prog × S.state := ⟨s.1.1, s.2.1⟩
-def prod.π₂ (s : S.prod.prog × S.prod.state) : S.prog × S.state := ⟨s.1.2, s.2.2⟩
-def prod.mk (sₗ sᵣ : S.prog × S.state) : S.prod.prog × S.prod.state := ⟨⟨sₗ.1, sᵣ.1⟩, ⟨sₗ.2, sᵣ.2⟩⟩
-
-/-- Relational soundness of the product semantics: If every stuck product trace of at most (2n) steps
-satisfies Φ, then for every pair of stuck traces of at most n steps, the relation holds on their stuck values. -/
-theorem prod.satisfies_soundness_fin {n : Nat} :
-    S.prod.satisfiesN Φ (n + n) c →
-    ∀ mₗ mᵣ cₗ cᵣ,
-      mₗ < n → mᵣ < n →
-      S.stuck cₗ → S.stuck cᵣ →
-      S.stepN mₗ (prod.π₁ c) cₗ → S.stepN mₗ (prod.π₂ c) cᵣ →
-      Φ (prod.mk cₗ cᵣ) :=
-  sorry
-
-end prod
--/
-
 
 /-- All traces of a configuration do not terminate. -/
 def nonterminating {S : SmallStep} (c : S.prog × S.state) : Prop :=
@@ -156,8 +73,27 @@ def nonterminating {S : SmallStep} (c : S.prog × S.state) : Prop :=
 def safe {S : SmallStep} (c : S.prog × S.state) : Prop :=
   ∀ n c', S.stepN n c c' → S.stuck c' → (S.to_val c').isSome
 
+def det_stepN_unqiue [Det S] {n} : S.stepN n c c' ∧ S.stepN n c c'' → c' = c'' := by
+  revert c
+  induction n
+  · intro _; rintro ⟨(H|_), (H'|_)⟩; exact H.symm.trans H'
+  · rename_i n IH
+    rintro c ⟨(_|⟨H1, H2⟩), (_|⟨H3, H4⟩)⟩
+    exact IH ⟨(Det.step_det H1 _ H3) ▸ H2, H4⟩
+
+/-- For all programs, they either surely teminate, or they don't. -/
+theorem SmallStep.termination_em {S : SmallStep} c : (∃ n, ∃ c', S.stepN n c c' ∧ S.stuck c') ∨ S.nonterminating c := by
+  refine (Classical.em _).elim .inr (fun H => .inl ?_)
+  simp only [nonterminating, Classical.not_forall, not_imp, Classical.not_not] at H
+  rcases H with ⟨n, c', H, Hs⟩
+  exists n
+  exists c'
+
 /-- A conservative definition of program equivalence, which should work as long as our semantics
-is deterministic. -/
+is deterministic.
+
+This is the thing we eventually want to prove about our programs.
+-/
 def PRel {S : SmallStep}
     (Φi : (S.prog × S.state) → (S.prog × S.state) → Prop)
     (Φf : S.val → S.val → Prop) : Prop :=
@@ -194,6 +130,15 @@ def Rel.lift2 {S : SmallStep} (p : S.prog) (Rs : S.state → Prop) (c1 c2 : S.pr
 /-- The trivial relation on configurations. -/
 def Rel.triv {T : Type _} (_ _ : T) : Prop := True
 
+/-- One relation is implied by another.
+
+markusde: use this for the static parts of verification, eg. allocation and value of input tensors in HBM.
+-/
+def Rel.implies {T : Type _} (R1 R2 : T → T → Prop) : Prop := ∀ t1 t2, R1 t1 t2 → R2 t1 t2
+
+theorem Rel.implies_triv {T : Type _} (R : T → T → Prop) : Rel.implies R Rel.triv :=
+  fun _ _ _ => trivial
+
 /-- If a program is related to itself with
  - The "equality" starting relation
  - the trivial terminal relation,
@@ -209,7 +154,245 @@ theorem PRel.safety {S : SmallStep} p (R : S.state → Prop) (Hp : PRel (Rel.lif
   rcases (Hval cf cf n n ⟨Hstep, Hstuck, Hstep, Hstuck⟩) with ⟨v1, _, Hv1, _, _⟩
   rw [Hv1]; rfl
 
+/-- A relation between two programs such that: Φi holds for everything the left program can step to -/
+def Rel.bind_l {S : SmallStep} (Φi : (S.prog × S.state) → (S.prog × S.state) → Prop)
+  (cl cr : S.prog × S.state) : Prop := ∀ cl', S.step cl cl' -> Φi cl' cr
+
+/-- A relation between two programs such that: Φi holds for everything the left program can step to -/
+def Rel.bind_r {S : SmallStep} (Φi : (S.prog × S.state) → (S.prog × S.state) → Prop)
+  (cl cr : S.prog × S.state) : Prop := ∀ cr', S.step cr cr' -> Φi cl cr'
+
+/-- Lift a relation on values to a relation on configurations, asserting that:
+ - both configurations are values,
+ - Φf holds on their values. -/
+def Rel.lift_values {S : SmallStep} (Φf : S.val → S.val → Prop)
+    (cl cr : S.prog × S.state) : Prop := ∃ vl vr, S.to_val cl = some vl ∧ S.to_val cr = some vr ∧ Φf vl vr
+
+theorem Rel.lift_values_mono {S : SmallStep}  {Φ1 Φ2 : S.val → S.val → Prop}
+    (H : Rel.implies Φ1 Φ2) : Rel.implies (Rel.lift_values Φ1) (Rel.lift_values Φ2) := by
+  intro c1 c2 Hl
+  rcases Hl with ⟨v1, v2, Hv1, Hv2, Hv12⟩
+  exact ⟨v1, v2, Hv1, Hv2, H _ _ Hv12⟩
+
+def Rel.both (P : T → Prop) (t1 t2 : T) : Prop := P t1 ∧ P t2
+
+theorem Rel.lift_values_triv_stuck_left {S : SmallStep} (cl cr : S.prog × S.state)
+    (H : Rel.lift_values Rel.triv cl cr) : S.stuck cl := by
+  rcases H with ⟨v, _, Hv, _, _⟩; intro Hs; apply Hv ▸ S.value_stuck; rfl
+
+theorem Rel.lift_values_triv_stuck_right {S : SmallStep} (cl cr : S.prog × S.state)
+    (H : Rel.lift_values Rel.triv cl cr) : S.stuck cr := by
+  rcases H with ⟨_, v, _, Hv, _⟩; intro Hs; apply Hv ▸ S.value_stuck; rfl
+
+theorem Rel.lift_values_triv_stuck_both {S : SmallStep} (cl cr : S.prog × S.state)
+  (H : Rel.lift_values Rel.triv cl cr) : Rel.both (S.stuck ·) cl cr :=
+  ⟨Rel.lift_values_triv_stuck_left cl cr H, Rel.lift_values_triv_stuck_right cl cr H⟩
+
+/-- If either program is not stuck, the Rel.lift_values relation cannot hold. -/
+theorem rel_lift_values_not_stuck {S : SmallStep} (cl cr : S.prog × S.state) {Φ}
+    (H : ¬S.stuck cl ∨ ¬S.stuck cr) : ¬Rel.lift_values Φ cl cr := by
+  rintro ⟨vl, vr, Hl, Hr, _⟩
+  apply H.elim
+  · intro H
+    apply H
+    intro c
+    apply Hl ▸ S.value_stuck (c := cl)
+    rfl
+  · intro H
+    apply H
+    intro c
+    apply Hr ▸ S.value_stuck (c := cr)
+    rfl
+
+/-- If either program is nonterminating, the Rel.lift_values relation cannot hold.
+TODO: Use rel_lift_values_not_stuck
+-/
+theorem rel_lift_values_not_nonterminating {S : SmallStep} (cl cr : S.prog × S.state) {Φ}
+    (H : nonterminating cl ∨ nonterminating cr) : ¬Rel.lift_values Φ cl cr := by
+  rintro ⟨vl, vr, Hl, Hr, _⟩
+  apply H.elim
+  · intro H
+    apply (H 0 cl (stepN.done rfl))
+    intro _
+    apply Hl ▸ S.value_stuck
+    rfl
+  · intro H
+    apply (H 0 cr (stepN.done rfl))
+    intro _
+    apply Hr ▸ S.value_stuck
+    rfl
+
+-- def Rel.both_stuck {S : SmallStep} (cl cr : S.prog × S.state) : Prop := S.stuck cl ∧ ¬S.stuck cr
+
+-- /-- A relation between two programs such that:
+--   - Both programs can take a step, and Φi holds for everything that both programs can step to, or
+--   - Both programs are stuck, and Φf holds for their stuck values.-/
+-- def Rel.bind_lr_sync {S : SmallStep} (Φi : (S.prog × S.state) → (S.prog × S.state) → Prop) (Φf : S.val → S.val → Prop)
+--   (cl cr : S.prog × S.state) : Prop :=
+--     (Rel.lift_values Φf cl cr) ∨
+--     (Rel.both (¬S.stuck ·) cl cr ∧ ∀ cl' cr', S.step cl cl' → S.step cr cr' → Φi cl cr)
+
+/- A step-indexed version of PRel.
+
+Both programs need to either terminate in values satisfying Φf in at most n steps,
+or take at least n steps.
+-/
+def PRelN {S : SmallStep} (n : Nat) (Φi : (S.prog × S.state) → (S.prog × S.state) → Prop) (Φf : S.val → S.val → Prop) : Prop :=
+  match n with
+  | 0 => True
+  | .succ n' =>
+      -- For any two initial states that are related by Φi
+      ∀ c1 c2, Φi c1 c2 →
+      -- Either they are both values, and satisfy Φf
+      (Rel.lift_values Φf c1 c2) ∨
+      -- or, there exist target states c1' c2
+      -- such that the left and right sides can both take >1 steps to reach the target states
+      (∃ n1 n2 : Nat, ∃ c1' c2',
+          S.stepN n1.succ c1 c1' ∧
+          S.stepN n2.succ c2 c2' ∧
+          PRelN n' (fun ρ1 ρ2 => ρ1 = c1' ∧ ρ2 = c2) Φf)
+
+/-- Property of the global state which is true at every point during execution. -/
+def strong_relational_invariant {S : SmallStep} (Φi : S.prog × S.state → S.prog × S.state → Prop) : Prop :=
+    (∀ cl cr cl' : S.prog × S.state, Φi cl cr → S.step cl cl' → Φi cl' cr) ∧
+    (∀ cl cr cr' : S.prog × S.state, Φi cl cr → S.step cr cr' → Φi cl cr')
+
+-- TODO: Cleanup
+theorem stepN_add_iff {S : SmallStep} {n1 n2 : Nat} {c1 c2} :
+    S.stepN (n1 + n2) c1 c2 ↔ ∃ c3, S.stepN n1 c1 c3 ∧ S.stepN n2 c3 c2 := by
+  revert n2 c1 c2
+  induction n1
+  · intro n2 c1 c2
+    rw [Nat.add_comm]
+    constructor
+    · rw [Nat.add_zero]
+      intro H
+      exists c1
+      exact ⟨stepN.done rfl, H⟩
+    · rintro ⟨c3, ⟨He⟩, _⟩
+      rw [Nat.add_zero, He]
+      trivial
+  · rename_i n1 IH; intro n2 c1 c2
+    constructor
+    · rw [Nat.add_right_comm n1 1 n2]
+      intro H
+      rcases H
+      rename_i c3 Hstep Hrest
+      rcases IH.mp Hrest with ⟨x, y, z⟩
+      exists x
+      constructor
+      · apply stepN.step Hstep y
+      · apply z
+    · rw [Nat.add_right_comm n1 1 n2]
+      rintro ⟨c3, x, y⟩
+      rcases x
+      rename_i a b c
+      apply stepN.step b
+      apply IH.mpr
+      exists c3
+
+-- Note: This theorem is not true in the presence of nondeterminism because
+-- nonterminating (Ω | 0) and step (Ω | 0) 0 but not nonterminating 0
+theorem nonterminating_step [Det S] {c c'} (Hn : nonterminating c) (Hs : S.step c c') :
+    nonterminating c' := by
+  intro n c'' Hs'
+  apply Hn n.succ
+  rw [Nat.succ_eq_one_add]
+  apply stepN_add_iff.mpr
+  exists c'
+  exact ⟨stepN.step Hs (stepN.done rfl), Hs'⟩
+
+
+/- Deterministic programs which satisfy PRelN for all n must be equiterminating.
+
+Note: We require that Φi behaves like a relational invariant on the state. This can encode things
+like input tensor values, which we will be a hypothesis of our adequacy statement. -/
+theorem PRelN_terminating [Det S] {Φi Φf} {cl cr} (HΦ : Φi cl cr) (Hterm : nonterminating cl)
+    (HInv : strong_relational_invariant Φi) (Hrel : ∀ n, PRelN (S := S) n Φi Φf) : nonterminating cr := by
+  -- Sketch: (Rel.lift_values Φf c1 c2) will never be true, so PRelN gets unfolded at least N times.
+  -- This means that cr will take at least (gas + 1) steps, so executing to (gas) will not be stuck.
+  intro gas
+  revert cl cr
+  induction gas
+  · intro cl cr HΦ Hterm
+    have Hrel' := Hrel 1
+    simp only [PRelN] at Hrel'
+    have Hrel'' := Hrel' cl cr HΦ; clear Hrel'
+    intro c' Hstep0 Hstuck
+    rcases Hrel'' with (H|⟨n1, n2, c1', c2', H1, H2, _⟩)
+    · exact rel_lift_values_not_nonterminating cl cr (.inl Hterm) H
+    · rcases Hstep0 with ⟨Heq⟩
+      rcases H2
+      rename_i _ HK _
+      rw [←Heq] at Hstuck
+      exact Hstuck _ HK
+  · rename_i gas IH
+    intro cl cr HΦ Hterm
+    rintro c ⟨⟩; rename_i c' Hs Hsn
+    -- Use Hrel to unfold once
+    have Hrel' := Hrel (gas + 1) cl cr HΦ <;> clear Hrel
+    rcases Hrel' with (H|⟨n1, n2, c1', c2', H1, H2, _⟩)
+    · intro Hk
+      apply rel_lift_values_not_stuck _ _ _ H
+      right
+      exact fun a => a c' Hs
+    -- By H1 and H2, both the left and right hadn sides can take at least 1 step.
+    rcases stepN_add_iff.mp (Nat.succ_eq_one_add n1 ▸ H1) with ⟨cl_next, Hstep_l, Hrest_l⟩
+    rcases stepN_add_iff.mp (Nat.succ_eq_one_add n2 ▸ H2) with ⟨cr_next, Hstep_r, Hrest_r⟩
+    -- By HInv, Φi holds of their left and right sides
+    have Hinv : Φi cl_next cr_next := by
+      apply HInv.1 _ _ _ _ (S.stepN_one Hstep_l)
+      apply HInv.2 _ _ _ _ (S.stepN_one Hstep_r)
+      exact HΦ
+    -- By Hterm, the new left branch is still nonterminating
+    have Hnt : nonterminating cl_next := nonterminating_step Hterm (S.stepN_one Hstep_l)
+    -- Reassociate Hs and Hsn to get that the new step takes gas steps to get to c' (det?)
+    have Hrec : S.stepN gas cr_next c := by
+      have Hstep_r' := S.stepN_one Hstep_r
+      rw [← Det.step_det Hstep_r' c' Hs]
+      exact Hsn
+    exact IH Hinv Hnt _ Hrec
+
+
+
+/-- Soundness of the step-indexed relation.
+If we can prove that the relation holds for all finite traces, then PRel holds between our programs. -/
+theorem PRelN_PRel [Det S] {Φi Φf} (HInv : strong_relational_invariant Φi) :
+    (∀ n, PRelN (S := S) n Φi Φf) → PRel (S := S) Φi Φf := by
+  intro HP c1 c2 HΦi
+  rcases SmallStep.termination_em c1 with (Hc1 | Hc1) <;>
+  rcases SmallStep.termination_em c2 with (Hc2 | Hc2)
+  · -- Both programs terminate.
+    constructor
+    · -- False equiv valse
+      sorry
+    · -- Prove: That for any two possible stuck states that we eventually step to,
+      -- they are values where Φf holds.
+      -- intro c1' c2' n m ⟨H1, H2, H3, H4⟩
+      -- have HP' := HP (Nat.max n m)
+      sorry
+  · exfalso
+    -- TOOD: Cleanup the PRelN_terminating proof and apply it in the other direction
+    sorry
+  · exfalso
+    have HN : (nonterminating c2) := PRelN_terminating HΦi Hc1 HInv HP
+    rcases Hc2 with ⟨n, c', H1, H2⟩
+    exact HN n c' H1 H2
+  · constructor
+    · simp_all
+    ·
+      rintro c1' c2' n m ⟨H1, H2, H3, H4⟩
+      exfalso
+      -- Nonterminating can't step to a stuck state
+      sorry
+
 namespace SmallStep
+
+
+
+
+
+/- Below: Junk -/
 
 
 /-
@@ -266,4 +449,128 @@ def lift_rel (R : Val × State → Val × State → Prop) (p1 p2 : Pgm × State)
 -- steps and right steps.
 
 end Product
+-/
+
+/-
+
+Stuff for when I was trying an explicit product semantics:
+
+/-- For any of the first n steps of execution, all stuck states satisfy `Φ`. -/
+inductive satisfiesN (Φ : S.prog × S.state → Prop) : Nat → S.prog × S.state → Prop where
+| stuck : S.stuck c → Φ c → satisfiesN Φ n c
+| step  : S.step c c' → satisfiesN Φ n c' → satisfiesN Φ n.succ c
+
+theorem satisfiesN_stepN (H : S.satisfiesN Φ n c) : ∀ m, m ≤ n → S.stuck c' → S.stepN m c c' → Φ c' := by
+  revert c
+  induction n
+  · intro c H m Hm Hs Hs'
+    rw [Nat.le_zero_eq] at Hm
+    rcases H with ⟨_, H⟩
+    exact (stepN_zero_inv S (Hm▸Hs'))▸H
+  rename_i n IH
+  rintro c H m Hm Hstuck Hstep
+  cases H
+  · rename_i Hs' HΦ
+    have Hz := stepN_stuck_inv S Hstep Hs'
+    have Hc := stepN_zero_inv S (Hz ▸ Hstep)
+    exact Hc ▸ HΦ
+  rename_i _ Hsat Hstep'
+  rcases m with (_|m)
+  · exact Hstuck _ (stepN_zero_inv S Hstep ▸ Hstep') |>.elim
+  -- have Hm' := Nat.add_le_add_iff_right ▸ Hm
+  cases Hstep
+  -- apply IH Hsat _ (Nat.le_of_lt_succ Hm) Hstuck
+  sorry
+-/
+
+/-
+
+Product semantics stuff
+
+
+@[simp] abbrev prod.prog (S : SmallStep) := S.prog × S.prog
+@[simp] abbrev prod.state (S : SmallStep) := S.state × S.state
+@[simp] abbrev prod.val (S : SmallStep) := S.val × S.val
+
+inductive prod.step {S : SmallStep} : (prod.prog S) × (prod.state S) → (prod.prog S) × (prod.state S) → Prop where
+| step_l : S.step (p1, s1) (p1', s1') → prod.step ((p1, p2), (s1, s2)) ((p1, p2'), (s1, s2'))
+| step_r : S.step (p2, s2) (p2', s2') → prod.step ((p1, p2), (s1, s2)) ((p1, p2'), (s1, s2'))
+
+@[simp] def prod.to_val {S : SmallStep} (c : prod.prog S × prod.state S) : Option (prod.val S) :=
+  match S.to_val ⟨c.1.1, c.2.1⟩, S.to_val ⟨c.1.2, c.2.2⟩ with
+  | some v1, some v2 => some (v1, v2)
+  | _, _ => none
+
+theorem prod.value_stuck {S : SmallStep} {c c' : prod.prog S × prod.state S} :
+    (prod.to_val c).isSome → prod.step c c' → False := by
+  rcases c with ⟨⟨p1, p2⟩, ⟨s1, s2⟩⟩
+  simp only [to_val]
+  split
+  · rename_i Hv1 Hv2
+    intro _ Hstep; rcases Hstep with (Hs|Hs)
+    · exact S.value_stuck (Hv1▸rfl) Hs
+    · exact S.value_stuck (Hv2▸rfl) Hs
+  · simp
+
+def prod (S : SmallStep) : SmallStep where
+  prog := prod.prog S
+  state := prod.state S
+  val := prod.val S
+  step := prod.step
+  to_val := prod.to_val
+  value_stuck := prod.value_stuck
+
+-/
+
+/- I think I actually need this to be in the step-indexed relation...
+
+-- If we can prove a PRel starting from Rel.bind_lr_sync, then either
+-- both programs are stuck, or both programs make progress and satisfy PRel Φj
+-- Then, we can define weakestpre by Rel.bind_lr_sync (or a stuttering variant) and
+-- use this in the adequacy proof.
+theorem PRel.bind_lr_sync {S : SmallStep} {c1 c2 : S.prog × S.state}
+    {Φi Φj : (S.prog × S.state) → (S.prog × S.state) → Prop}
+    -- If c1 and c2 only ever step from states related by Φi to states related by Φj,
+    (Hij : ∀ c1' c2', S.step c1 c1' → S.step c2 c2' → Φi c1 c2 → Φj c1 c2)
+    -- And we have established that programs are Φj-related
+    {Φf : S.val → S.val → Prop} :
+    -- And we have established
+    PRel (Rel.bind_lr_sync Φi Φf) Φf →
+    Φi c1 c2 →
+      ((Rel.lift_values Φf) c1 c2) ∨
+      (Rel.both (¬S.stuck ·) c1 c2 ∧ PRel (fun c1' c2' => S.step c1 c1' → S.step c2 c2' → Φi c1' c2') Φf)
+    := sorry
+-/
+
+/-
+
+
+section prod
+
+variable {S : SmallStep}
+
+
+/-- Every n-step trace in the product semantics can be thought of as two traces in the semantics
+of the components. -/
+theorem prod.step_noninterference {n : Nat} :
+    S.prod.stepN n ((p, q), (s, t)) ((p', q'), (s', t')) ↔
+    (∃ mₗ mᵣ : Nat, n = mₗ + mᵣ ∧ S.stepN mₗ (p, s) (p', s') ∧ S.stepN mᵣ (q, t) (q', t')) :=
+  sorry
+
+def prod.π₁ (s : S.prod.prog × S.prod.state) : S.prog × S.state := ⟨s.1.1, s.2.1⟩
+def prod.π₂ (s : S.prod.prog × S.prod.state) : S.prog × S.state := ⟨s.1.2, s.2.2⟩
+def prod.mk (sₗ sᵣ : S.prog × S.state) : S.prod.prog × S.prod.state := ⟨⟨sₗ.1, sᵣ.1⟩, ⟨sₗ.2, sᵣ.2⟩⟩
+
+/-- Relational soundness of the product semantics: If every stuck product trace of at most (2n) steps
+satisfies Φ, then for every pair of stuck traces of at most n steps, the relation holds on their stuck values. -/
+theorem prod.satisfies_soundness_fin {n : Nat} :
+    S.prod.satisfiesN Φ (n + n) c →
+    ∀ mₗ mᵣ cₗ cᵣ,
+      mₗ < n → mᵣ < n →
+      S.stuck cₗ → S.stuck cᵣ →
+      S.stepN mₗ (prod.π₁ c) cₗ → S.stepN mₗ (prod.π₂ c) cᵣ →
+      Φ (prod.mk cₗ cᵣ) :=
+  sorry
+
+end prod
 -/
